src/SoftBound/sb_db_trans.v
@@ -18,6 +18,7 @@ Require Import Metatheory.
 Require Import Znumtheory.
 Require Import sb_def.
 Require Import symexe_def.
+Require Import sub_symexe.
 Require Import sb_tactic.
 Require Import sub_tv.
 Require Import sb_db_pp.
@@ -26,6 +27,7 @@ Module SBpass.
 
 Export LLVMsyntax.
 Export LLVMgv.
+Export SimpleSE.
 
 Definition i8 := typ_int Size.Eight.
 Definition i32 := typ_int Size.ThirtyTwo.
@@ -600,7 +602,7 @@ end.
 
 Definition trans_fdef nts (f:fdef) : option fdef :=
 let '(fdef_intro (fheader_intro fa t fid la va) bs) := f in
-if SimpleSE.isCallLib fid then Some f
+if SBSE.isCallLib fid then Some f
 else
   let ex_ids := getFdefLocs f in
   match gen_metadata_fdef nts ex_ids nil f with
