src/TV/sub_tv_correct.v
@@ -15,10 +15,7 @@ Require Import ssa_dynamic.
 Require Import genericvalues.
 Require Import opsem_pp.
 Require Import trace.
-Require Import symexe_def.
-Require Import symexe_lib.
-Require Import symexe_complete.
-Require Import symexe_sound.
+Require Import sub_symexe.
 Require Import alist.
 Require Import ssa_props.
 Require Import sub_tv_def.
