src/TV/symexe_sound.v
@@ -337,8 +337,7 @@ Proof.
     apply wrong_assumption1 with (M2:=Mem1) in H12.
     split; eauto.
 
-  Case "insn_call".
-    admit.
+  Case "insn_call". inversion nc.
 Qed.
 
 Lemma aux__se_cmd__denotes__op_cmd : forall TD c nc lc als gl Mem1 lc' als' Mem2 lc0 als0 Mem0 sstate1 tr1 tr2,
@@ -380,7 +379,7 @@ Proof.
     simpl. auto.   
 
     destruct c; simpl; auto.
-      admit.
+      inversion nc.
 
     apply init_denotes_id; auto.
 Qed.
@@ -394,7 +393,7 @@ Proof.
   destruct c; intros nc id0 id1 st0 smap1 smem1 sframe1 seffects1 Hbinds 
                      HgetCmdLoc id0_isnt_id1; simpl;
     simpl in HgetCmdLoc; subst; auto using binds_updateAddAL_neq.
-    admit.
+    inversion nc.
 Qed.
   
 Lemma binds_se_cmds_onlyif : forall nbs i0 st0 smap1 smem1 sframe1 seffects1 c nc,
@@ -426,9 +425,9 @@ Proof.
       destruct nbranching_cmd0; simpl in HeqR; inversion HeqR; subst; 
         try solve [
           auto | 
-          apply binds_updateAddAL_neq; auto
+          apply binds_updateAddAL_neq; auto |
+          inversion notcall0
         ].
-        admit.
 Qed.
          
 Lemma binds_se_cmds_strengthen : forall nbs i1 st1 smap1 smem1 sframe1 seffects1,
@@ -442,9 +441,9 @@ Proof.
     destruct nbranching_cmd0; simpl in *; try solve [
       apply IHnbs in Binds; auto using updateAddAL_uniq;
         apply updateAddAL_inversion in Binds; auto;
-        destruct Binds as [[_ J] | [EQ1 EQ2]]; subst; try solve [auto|contradict i1_notin; auto]
+        destruct Binds as [[_ J] | [EQ1 EQ2]]; subst; try solve [auto|contradict i1_notin; auto] |
+      inversion notcall0
      ].
-     admit.
 Qed.
 
 Lemma binds_se_cmds_weaken : forall nbs i1 st1 smap1 smem1 sframe1 seffects1,
@@ -457,9 +456,9 @@ Proof.
     destruct a.
     destruct nbranching_cmd0; simpl; try solve [
       simpl in i1_notin;
-      apply IHnbs; auto using updateAddAL_uniq, binds_updateAddAL_neq
+      apply IHnbs; auto using updateAddAL_uniq, binds_updateAddAL_neq |
+      inversion notcall0 
       ].
-      admit.
 Qed.
 
 Lemma _binds_se_cmds_if : forall nbs i1 st1 smap1 smem1 sframe1 seffects1 i0 st0,
@@ -513,9 +512,9 @@ Proof.
       destruct nbranching_cmd0; simpl in HeqR; inversion HeqR; subst; 
         try solve [
           auto | 
-          eapply _binds_se_cmds_if; eauto
+          eapply _binds_se_cmds_if; eauto |
+          inversion notcall0
         ].
-        admit.
 Qed.
 
 Lemma binds_se_cmds : forall i0 st0 smap1 smem1 sframe1 seffects1 nbs c nc,
@@ -624,7 +623,7 @@ Proof.
                      (value2Sterm st.(STerms) v0)
                      (value2Sterm st.(STerms) v1)). auto.
 
-    admit.
+    inversion nc.
 Qed.
 
 Lemma in_se_cmds__prefix_last : forall nbs c nc id' smem1 sframe1 seffects1 i0,
@@ -1610,7 +1609,7 @@ Proof.
 
             rewrite lookupAL_rollbackAL_neq with (id0:=i0)(lc0:=lc0) in id'_in_env2; auto.
 
-  Case "insn_call". admit.
+  Case "insn_call". inversion nc.
 Qed. 
 
 Lemma se_cmds_denotes__composes__prefix_last__case1 : forall TD lc0 gl Mem0 nbs lc1 lc2 Mem1 id' c nc i0 st0,
@@ -2312,7 +2311,7 @@ Proof.
     split. inversion Hsframe_denotes2; subst; auto.
            inversion Hseffects_denote1; inversion Hseffects_denote2; subst; auto.
 
-  Case "insn_call". admit.
+  Case "insn_call". inversion nc.
 Qed.
 
 Definition se_cmds_denotes__decomposes__app_prop (nbs2:list nbranch) :=
